{
 "cells": [
  {
   "cell_type": "markdown",
   "metadata": {},
   "source": [
    "# Worked solutions 1"
   ]
  },
  {
   "cell_type": "markdown",
   "metadata": {},
   "source": [
    "This document contains sketch notes to some of the quiz questions. It is not comprehensive. We have tried to include most of the questions where it may not be obvious how to get to the correct answer. "
   ]
  },
  {
   "cell_type": "markdown",
   "metadata": {},
   "source": [
    "## Quiz 1\n",
    "\n",
    "### Question 15 \n",
    "\n",
    "$$\n",
    "\\begin{align*}\n",
    " ln\\left(   \\prod_{i=1}^n p^{x_i} (1-p)^{y_i} \\right)\n",
    " &=  ln\\left(  (p^{x_1} (1-p)^{y_1}) \\times (p^{x_2} (1-p)^{y_2}) \\times ... \\times (p^{x_n} (1-p)^{y_n}) \\right) \\\\\n",
    " &= ln(p^{x_1} (1-p)^{y_1}) + ln(p^{x_2} (1-p)^{y_2}) + ... + ln(p^{x_n} (1-p)^{y_n}) \\\\\n",
    "& = \\sum_{i=}^n ln( p^{x_i} (1-p)^{y_i})\n",
    "\\end{align*}\n",
    "$$\n",
    "\n",
    "We have\n",
    "\n",
    "$$\n",
    "\\begin{align*}\n",
    "ln(p^{x_1} (1-p)^{y_1}) & = ln(p^{x_1}) + ln(1-p)^{y_1}) \\\\\n",
    "& = x_1 ln(p) + y_1 ln(1-p)\n",
    "\\end{align*}\n",
    "$$\n",
    "\n",
    "Doing that to each term gives\n",
    "\n",
    "$$\n",
    "\\begin{align*}\n",
    " ln\\left(   \\prod_{i=1}^n p^{x_i} (1-p)^{y_i} \\right) & = \\sum_{i=}^n \\left( x_i ln(p) + y_i ln(1-p) \\right) \\\\\n",
    " & = \\sum_{i=}^n  x_i ln(p) + \\sum_{i=}^n y_i ln(1-p) \\\\\n",
    "\\end{align*}\n",
    "$$\n",
    "\n",
    "where we can split the summation into the two separate terms. Then,\n",
    "\n",
    "$$\n",
    "\\begin{align*}\n",
    " ln\\left(\\prod_{i=1}^n p^{x_i} (1-p)^{y_i} \\right) & = \\sum_{i=}^n  x_i ln(p) + \\sum_{i=}^n y_i ln(1-p) \\\\\n",
    " & = (x_1 ln(p) + x_2 ln(p) + ... + x_n ln(p)) + (y_1 ln(1-p) + y_2 ln(1-p) + ... + y_n ln(1-p)) \\\\\n",
    "  & = ln(p) (x_1 + x_2  + ... + x_n) + ln(1-p) (y_1 + y_2 + ... + y_n) \\\\\n",
    "  & = ln(p) \\sum_{x=1}^n x_i + ln(1-p) \\sum_{i=1}^n y_i\n",
    "\\end{align*}\n",
    "$$"
   ]
  },
  {
   "cell_type": "markdown",
   "metadata": {},
   "source": [
    "## Quiz 2\n",
    "\n",
    "### Question 3\n",
    "\n",
    "Differentiate\n",
    "\n",
    "$$\n",
    "\\begin{align*}\n",
    "f(x) = \\sqrt{1+x^2} \n",
    "\\end{align*}\n",
    "$$\n",
    "\n",
    "$$\n",
    "\\begin{align*}\n",
    "\\frac{d f(x)}{dx} & = \\frac{d  }{dx} (\\sqrt{1+x^2} ) \\\\\n",
    "\\end{align*}\n",
    "$$\n",
    "\n",
    "If we let $u=(1+x^2)$ then $f(x)=u^{1/2}$.\n",
    "\n",
    "$$\n",
    "\\begin{align*}\n",
    "\\frac{d f(x)}{dx} & = \\frac{df}{du} \\frac{du}{dx} \\\\ & = \\frac{d}{du} (u^{1/2}) \\times  \\frac{du}{dx}  \\\\ & = \\frac{1}{2} u^{-1/2} \\frac{du}{dx}\n",
    "\\end{align*}\n",
    "$$\n",
    "\n",
    "Now differentiating $u=(1+x^2)$ with respect to $x$ gives\n",
    "\n",
    "$$\n",
    "\\frac{du}{dx} = 2x\n",
    "$$\n",
    "\n",
    "Then\n",
    "\n",
    "$$\n",
    "\\begin{align*}\n",
    "\\frac{d f(x)}{dx} & =\\frac{1}{2} (1+x^2)^{-1/2} \\times 2x\n",
    "\\end{align*}\n",
    "$$\n",
    "\n",
    "which simplifies to give\n",
    "\n",
    "$$\n",
    "\\begin{align*}\n",
    "\\frac{d f(x)}{dx} & = \\frac{x}{\\sqrt{1+x^2}}\n",
    "\\end{align*}\n",
    "$$"
   ]
  },
  {
   "cell_type": "markdown",
   "metadata": {},
   "source": [
    "### Question 3\n",
    "\n",
    "Differentiate\n",
    "\n",
    "$$\n",
    "\\begin{align*}\n",
    "f(x) = \\frac{1}{log_e(x)} \n",
    "\\end{align*}\n",
    "$$\n",
    "\n",
    "Let $u=log_e(x)$. Then $f(x) = u^{-1}$\n",
    "\n",
    "$$\n",
    "\\begin{align*}\n",
    "\\frac{d f(x)}{dx} & = \\frac{df}{du} \\frac{du}{dx} \\\\ & = \\frac{d}{du} (u^{-1}) \\times  \\frac{du}{dx}  \\\\ & = - u^{-2} \\frac{du}{dx}\n",
    "\\end{align*}\n",
    "$$\n",
    "\n",
    "Now differentiating $u=log_e(x)$ with respect to $x$ gives\n",
    "\n",
    "$$\n",
    "\\frac{du}{dx} = \\frac{1}{x}\n",
    "$$\n",
    "\n",
    "Then\n",
    "\n",
    "$$\n",
    "\\begin{align*}\n",
    "\\frac{d f(x)}{dx} & = - (log_e(x))^{-2} \\frac{1}{x} \\\\ & = \\frac{-1}{x (log_e(x))^2}\n",
    "\\end{align*}\n",
    "$$\n"
   ]
  },
  {
   "cell_type": "markdown",
   "metadata": {},
   "source": [
    "### Question 6\n",
    "\n",
    "Differentiate\n",
    "\n",
    "$$\n",
    "\\begin{align*}\n",
    "f(x) = \\frac{(1+x)}{x^2} \n",
    "\\end{align*}\n",
    "$$\n",
    "\n",
    "You can use the quotient rule. I tend to use the product rule. It comes to the same thing. \n",
    "\n",
    "Let $F(x) = 1+x$ and $L(x) = \\frac{1}{x^2}$. Then $f(x) = F(x) \\times L(x)$. So we have \n",
    "\n",
    "$$\n",
    "\\begin{align*}\n",
    "\\frac{df(x)}{dx} & = \\frac{d }{dx} (F(x) \\times L(x))  \\\\ &=   L(x) \\frac{d }{dx} F(x) + F(x)  \\frac{d }{dx} L(x) \n",
    "\\end{align*}\n",
    "$$\n",
    "\n",
    "Now\n",
    "\n",
    "$$\n",
    "\\begin{align*}\n",
    "\\frac{d}{dx} F(x) & = \\frac{d}{dx} (1+x) =  1 \n",
    "\\end{align*}\n",
    "$$\n",
    "\n",
    "$$\n",
    "\\begin{align*}\n",
    "\\frac{d}{dx} L(x) & = \\frac{d}{dx} \\frac{1}{x^2} =  \\frac{-2}{x^3} \n",
    "\\end{align*}\n",
    "$$\n",
    "\n",
    "Then\n",
    "\n",
    "$$\n",
    "\\begin{align*}\n",
    "\\frac{df(x)}{dx} & =  \\frac{1}{x^2} \\times 1  + (1+x) \\times \\frac{-2}{x^3}  \\\\ & =  \\frac{1}{x^2} \\left( 1 - \\frac{2(1+x)}{x}\\right) \\\\ & =   \\frac{1}{x^2}  \\left(\\frac{1}{x} (x - 2 - 2x) \\right) \\\\ & =  \\frac{-(2 + x)}{x^3} \n",
    "\\end{align*}\n",
    "$$"
   ]
  },
  {
   "cell_type": "markdown",
   "metadata": {},
   "source": [
    "### Question 8\n",
    "\n",
    "\n",
    "$$\n",
    "\\begin{align*}\n",
    "L = -\\frac{(x-\\mu)^2}{s} - log(s) \n",
    "\\end{align*}\n",
    "$$\n",
    "\n",
    "Differentiating $L$ with respect to $\\mu$ gives\n",
    "\n",
    "$$\n",
    "\\begin{align*}\n",
    "\\frac{dL}{d\\mu} & = \\frac{d}{d\\mu} \\left( -\\frac{(x-\\mu)^2}{s} - log(s)  \\right) \\\\ & = \\frac{d}{d\\mu}  - \\frac{(x-\\mu)^2}{s} - \\frac{d}{d\\mu} log(s)   \\\\ & = - \\frac{1}{s} \\frac{d}{d\\mu} (x-\\mu)^2 - 0 \\\\& - \\frac{1}{s} \\times 2(x-\\mu) \\times -1 \\\\ & = \\frac{2 (x-\\mu)}{s}\n",
    "\\end{align*}\n",
    "$$\n",
    "\n",
    "Differentiating $L$ with respect to $s$ gives\n",
    "\n",
    "$$\n",
    "\\begin{align*}\n",
    "\\frac{dL}{ds} & = \\frac{d}{ds} \\left( -\\frac{(x-\\mu)^2}{s} - log(s)  \\right) \\\\ & = \\frac{d}{ds}  - \\frac{(x-\\mu)^2}{s} - \\frac{d}{ds} log(s)   \\\\ & = - (x-\\mu)^2 \\frac{d}{ds}  \\frac{1}{s} - \\frac{1}{s} \\\\ & = - (x-\\mu)^2 \\times \\frac{-1}{s^2} - \\frac{1}{s}  \\\\ & = \\frac{(x-\\mu)^2}{s^2} - \\frac{1}{s}\n",
    "\\end{align*}\n",
    "$$\n",
    "\n",
    "To get the second derivatives, we differentiate again. For example,\n",
    "\n",
    "$$\n",
    "\\begin{align*}\n",
    "\\frac{d^2L}{d\\mu^2} & =  \\frac{d}{d\\mu} \\left\\{ \\frac{d L}{d\\mu}    \\right\\}   \\\\ & =  \\frac{d}{d\\mu} \\frac{2 (x-\\mu)}{s} \\\\ & = \\frac{-2}{s}\n",
    "\\end{align*}\n",
    "$$\n",
    "\n",
    "And\n",
    "\n",
    "$$\n",
    "\\begin{align*}\n",
    "\\frac{d^2L}{ds^2} & =  \\frac{d}{ds} \\left\\{ \\frac{d L}{ds}    \\right\\}   \\\\ & =  \\frac{d}{ds} \\left\\{  \\frac{(x-\\mu)^2}{s^2} - \\frac{1}{s}\\right\\}  \\\\ & = (x-\\mu)^2 \\frac{d}{ds} \\frac{1}{s^2} -  \\frac{d}{ds} \\frac{1}{s}  \\\\ & =  (x-\\mu)^2 \\times \\frac{-2}{s^3}  -   \\frac{-1}{s^2} \\\\ & =  \\frac{-2 (x-\\mu)^2}{s^3} + \\frac{1}{s^2}  \n",
    "\\end{align*}\n",
    "$$\n",
    "\n",
    "Finally, \n",
    "\n",
    "$$\n",
    "\\begin{align*}\n",
    "\\frac{d^2L}{d\\mu ds^2} & =  \\frac{d}{ds} \\left\\{ \\frac{d L}{d \\mu}  \\right\\}   \\\\ & =   \\frac{d}{ds} \\frac{2 (x-\\mu)}{s} \\\\ & = 2 (x-\\mu) \\frac{d}{ds} \\frac{1 }{s}  \\\\ & = 2 (x-\\mu) \\times \\frac{-1}{s^2}  \\\\ & = \\frac{-2 (x-\\mu)}{s^2}  \n",
    "\\end{align*}\n",
    "$$\n",
    "\n",
    "You can also do the other way round (differentiate first with respect to $s$ and then with respect to $\\mu$, but you come to the same answer). \n"
   ]
  },
  {
   "cell_type": "markdown",
   "metadata": {},
   "source": [
    "### Question 11\n",
    "\n",
    "$$\n",
    "\\begin{align*}\n",
    "\\int \\frac{x}{x^2 - 4} dx  \n",
    "\\end{align*}\n",
    "$$\n",
    "\n",
    "We notice that if we differentiate the denominator, we get $2x$, which is proportional to the numerator. Remember the rule \n",
    "\n",
    "$$ \n",
    "\\int \\frac{F'(x)}{F(x)} dx = log_e(F(x))\n",
    "$$\n",
    "\n",
    "So if we let $F(x) = x^2 - 4$ then \n",
    "\n",
    "$$\n",
    "\\begin{align*}\n",
    "\\int \\frac{2 x}{x^2 - 4} dx  = log_e(x^2 - 4)\n",
    "\\end{align*}\n",
    "$$\n",
    "\n",
    "which tells us that \n",
    "\n",
    "$$\n",
    "\\begin{align*}\n",
    "\\int \\frac{x}{x^2 - 4} dx  = \\frac{1}{2} log_e(x^2 - 4)\n",
    "\\end{align*}\n",
    "$$\n",
    "\n",
    "We can express this in various ways, \n",
    "\n",
    "$$\n",
    "\\begin{align*}\n",
    "\\int \\frac{x}{x^2 - 4} dx  & = \\frac{1}{2} log_e(x^2 - 4) \\\\ & = log_e( \\sqrt{x^2 - 4}) \\\\ & =  \\frac{1}{2} log_e((x-2)(x+2)) \n",
    "\\end{align*}\n",
    "$$\n",
    "\n",
    "The easiest way to tackle this question, however, is to differentiate the potential solutions and see which gives the correct answer! \n",
    "\n"
   ]
  },
  {
   "cell_type": "markdown",
   "metadata": {},
   "source": [
    "### Question 12\n",
    "\n",
    "(a) Area under curve $y=x^2$ between $x=0$ and $x=3$. \n",
    "\n",
    "This is\n",
    "\n",
    "$$\n",
    "\\begin{align*}\n",
    "\\int_0^3 x^2 dx  & = \\left[ \\frac{x^3}{3} \\right]_0^3 \\\\ & =  \\frac{3^3}{3}  -  \\frac{0^3}{3} \\\\ & = 9 - 0 = 9\n",
    "\\end{align*}\n",
    "$$\n",
    "\n",
    "(b) Area under curve $y=x^2$ between $x=-0$ and $x=-3$. \n",
    "\n",
    "This is\n",
    "\n",
    "$$\n",
    "\\begin{align*}\n",
    "\\int_{-3}^0 x^2 dx  & = \\left[ \\frac{x^3}{3} \\right]_{-3}^0 \\\\ & =  \\frac{0^3}{3}  -  \\frac{(-3)^3}{3} \\\\ & = 0 - (-9) = 9\n",
    "\\end{align*}\n",
    "$$\n"
   ]
  },
  {
   "cell_type": "markdown",
   "metadata": {},
   "source": [
    "### Question 13\n",
    "\n",
    "(a) Area under curve $y=x^3 - 3x$ between $x=0$ and $x=3$. \n",
    "\n",
    "This is\n",
    "\n",
    "$$\n",
    "\\begin{align*}\n",
    "\\int_0^3 (x^3 - 3x) dx  & = \\left[ \\frac{x^4}{4} - \\frac{3 x^2}{2} \\right]_0^3 \\\\ & =  \\frac{3^4}{4} - \\frac{3 . 3^2}{2}  -  \\frac{0^4}{4} +   \\frac{3 . 0^2}{2}  \\\\ & = \\frac{3^3}{2}  \\left( \\frac{3}{2} - 1\\right) \\\\ & =  \\frac{3^3}{4} = 6.75\n",
    "\\end{align*}\n",
    "$$\n",
    "\n",
    "(b) Area under curve $y=x^3 - 3x$ between $x=-2$ and $x=2$. \n",
    "\n",
    "This is\n",
    "\n",
    "$$\n",
    "\\begin{align*}\n",
    "\\int_{-2}^2 (x^3 - 3x) dx  & = \\left[ \\frac{x^4}{4} - \\frac{3 x^2}{2} \\right]_{-2}^2 \\\\ & =  \\left(\\frac{2^4}{4} - \\frac{3 . 2^2}{2}\\right)  -  \\left(\\frac{(-2)^4}{4} - \\frac{3 . (-2)^2}{2}\\right)   = 0 \n",
    "\\end{align*}\n",
    "$$"
   ]
  },
  {
   "cell_type": "markdown",
   "metadata": {},
   "source": [
    "## Quiz 3\n",
    "\n",
    "### Question 6\n",
    "\n",
    "$$\n",
    "\\begin{align*}\n",
    "A = \\begin{pmatrix} 1 &4 \\\\ 5 &1 \\\\ 2 &3 \\end{pmatrix}\n",
    "\\end{align*}\n",
    "$$\n",
    "\n",
    "$$\n",
    "\\begin{align*}\n",
    "B = \\begin{pmatrix} 4 &2 &1 \\\\ 3 &6 &3 \\\\ 2 & 5 & 5 \\end{pmatrix}\n",
    "\\end{align*}\n",
    "$$\n",
    "\n",
    "$$\n",
    "\\begin{align*}\n",
    "C = \\begin{pmatrix} 2&4 \\\\ 3 &1 \\\\ 6 &0 \\end{pmatrix}\n",
    "\\end{align*}\n",
    "$$\n",
    "\n",
    "$$\n",
    "\\begin{align*}\n",
    "A + C  =  \\begin{pmatrix} 1 &4 \\\\ 5 &1 \\\\ 2 &3 \\end{pmatrix} + \\begin{pmatrix} 2&4 \\\\ 3 &1 \\\\ 6 &0 \\end{pmatrix} = \n",
    " \\begin{pmatrix} 1+2 &4+4 \\\\ 5+3 &1+1 \\\\ 2+6 &3+0 \\end{pmatrix} = \n",
    " \\begin{pmatrix} 3 &8 \\\\ 8 &2 \\\\ 8 &3 \\end{pmatrix} \n",
    "  \\end{align*}\n",
    "$$\n",
    "\n",
    "$$\n",
    "\\begin{align*}\n",
    "A - C  =  \\begin{pmatrix} 1 &4 \\\\ 5 &1 \\\\ 2 &3 \\end{pmatrix} - \\begin{pmatrix} 2&4 \\\\ 3 &1 \\\\ 6 &0 \\end{pmatrix} = \n",
    " \\begin{pmatrix} 1-2 &4-4 \\\\ 5-3 &1-1 \\\\ 2-6 &3-0 \\end{pmatrix} = \n",
    " \\begin{pmatrix} -1 &0 \\\\ 2 &0 \\\\ -4 &3 \\end{pmatrix} \n",
    "  \\end{align*}\n",
    "$$\n",
    "\n",
    "$$\n",
    "\\begin{align*}\n",
    "A^T + C^T = (A+C)^T  =   \\begin{pmatrix} 3 &8 \\\\ 8 &2 \\\\ 8 &3 \\end{pmatrix} ^2 =  \\begin{pmatrix} 3 &8 &8 \\\\ 8 &2 &3 \\end{pmatrix}\n",
    "  \\end{align*}  \n",
    "$$ "
   ]
  },
  {
   "cell_type": "markdown",
   "metadata": {},
   "source": [
    "### Question 7\n",
    "  \n",
    "$$\n",
    "\\begin{align*}\n",
    "2 A = 2 \\times \\begin{pmatrix} 1 &4 \\\\ 5 &1 \\\\ 2 &3 \\end{pmatrix} =  \\begin{pmatrix} 2 \\times 1 &2 \\times 4 \\\\ 2 \\times 5 &2 \\times 1 \\\\ 2 \\times2 &2 \\times 3 \\end{pmatrix} =  \\begin{pmatrix} 2 &8 \\\\ 10 &2 \\\\ 4 &6 \\end{pmatrix}\n",
    "\\end{align*}\n",
    "$$\n",
    "\n",
    "$$\n",
    "\\begin{align*}\n",
    "-1(A-C)3  = -3 \\times (A-C) = -3 \\times  \\begin{pmatrix} -1 &0 \\\\ 2 &0 \\\\ -4 &3 \\end{pmatrix}  =   \\begin{pmatrix} -3 \\times -1 &-3 \\times 0 \\\\ -3 \\times 2 &-3 \\times 0 \\\\ -3 \\times -4 &-3 \\times 3 \\end{pmatrix}  =   \\begin{pmatrix} 3 &0 \\\\ -6  & 0 \\\\ 12 &-9 \\end{pmatrix} \n",
    "\\end{align*}\n",
    "$$"
   ]
  },
  {
   "cell_type": "markdown",
   "metadata": {},
   "source": [
    "### Question 9\n",
    "\n",
    "$$\n",
    "\\begin{align*}\n",
    "D = \\begin{pmatrix} 3 \\\\ -1 \\end{pmatrix}\n",
    "\\end{align*}\n",
    "$$\n",
    "\n",
    "$$\n",
    "\\begin{align*}\n",
    " A D = \\begin{pmatrix} 1 &4 \\\\ 5 &1 \\\\ 2 &3 \\end{pmatrix} \\times \\begin{pmatrix} 3 \\\\ -1 \\end{pmatrix} = \\begin{pmatrix} 1\\times 3 + 4\\times -1 \\\\ 5 \\times 3 + 1 \\times -1 \\\\ 2 \\times 3 + 3 \\times -1 \\end{pmatrix} =\\begin{pmatrix} 3 - 4 \\\\ 15 -1 \\\\ 6 - 3 \\end{pmatrix} =\\begin{pmatrix} -1 \\\\ 14 \\\\ 3 \\end{pmatrix}\n",
    "\\end{align*} \n",
    "$$"
   ]
  },
  {
   "cell_type": "markdown",
   "metadata": {},
   "source": [
    "### Question 10\n",
    "\n",
    "$$\n",
    "\\begin{align*}\n",
    "B A = \\begin{pmatrix} 4 &2 &1 \\\\ 3 &6 &3 \\\\ 2 & 5 & 5 \\end{pmatrix} \\begin{pmatrix} 1 &4 \\\\ 5 &1 \\\\ 2 &3 \\end{pmatrix} & = \\begin{pmatrix} 4 \\times 1 + 2\\times 5 + 1\\times 2 & 4 \\times 4 + 2\\times 1 + 1\\times 3 \\\\ 3\\times  1 + 6\\times  5+  3\\times 2 &3\\times  4 + 6\\times 1 + 3\\times 3 \\\\ 2\\times 1 +  5\\times 5 +  5\\times  2 &2\\times 4 +  5\\times 1 +  5\\times 3 \\end{pmatrix} \\\\ & = \\begin{pmatrix} 4 + 10 + 2 & 16 + 2 + 3  \\\\ 3 + 30 + 6 & 12 + 6 + 9 \\\\ 2 + 25 + 10 &8 + 5 + 15 \\end{pmatrix}  \\\\ & = \\begin{pmatrix} 16 &21  \\\\ 39 &27 \\\\ 37 &28 \\end{pmatrix}   \n",
    "\\end{align*}\n",
    "$$\n",
    "\n",
    "$AB$ is undefined. "
   ]
  },
  {
   "cell_type": "markdown",
   "metadata": {},
   "source": [
    "### Question 12\n",
    "\n",
    "$$\n",
    "\\begin{align*}\n",
    "E = \\begin{pmatrix} 2 &1 \\\\ -3 &0 \\end{pmatrix}\n",
    "\\end{align*}\n",
    "$$\n",
    "\n",
    "$$\n",
    "det(E) = 2 \\times 0 - (1 \\times -3) = 3\n",
    "$$"
   ]
  },
  {
   "cell_type": "markdown",
   "metadata": {},
   "source": [
    "### Question 13\n",
    "\n",
    "$$\n",
    "\\begin{align*}\n",
    "E^{-1} = \\frac{1}{det(E)}\\begin{pmatrix} 0 &-1 \\\\ 3 &2 \\end{pmatrix} = \\frac{1}{3}\\begin{pmatrix} 0 &-1 \\\\ 3 &2 \\end{pmatrix} = \\begin{pmatrix} 0 &-1/3 \\\\ 1 &2/3 \\end{pmatrix}\n",
    "\\end{align*}\n",
    "$$\n",
    "\n",
    "Check: \n",
    "\n",
    "$$\n",
    "\\begin{align*}\n",
    "E E^{-1} = \\begin{pmatrix} 2 &1 \\\\ -3 &0 \\end{pmatrix} \\begin{pmatrix} 0 &-1/3 \\\\ 1 &2/3 \\end{pmatrix} & = \\begin{pmatrix} 2 \\times 0 + 1 \\times 1 &2 \\times -1/3 + 1\\times 2/3  \\\\ -3 \\times 0 + 0 \\times 1 &-3 \\times -1/3 + 0 \\times 2/3  \\end{pmatrix}  \\\\ & = \\begin{pmatrix} 1 &0  \\\\ 0 &1 \\end{pmatrix} = I\n",
    "\\end{align*}\n",
    "$$\n",
    "\n",
    "as expected. "
   ]
  },
  {
   "cell_type": "markdown",
   "metadata": {},
   "source": [
    "### Question 14\n",
    "\n",
    "$$\n",
    "\\begin{align*}\n",
    "E^2 = \\begin{pmatrix} 2 &1 \\\\ -3 &0 \\end{pmatrix}\\begin{pmatrix} 2 &1 \\\\ -3 &0 \\end{pmatrix} = \\begin{pmatrix} 2 \\times 2 + 1 \\times -3 & 2 \\times 1 + 1 \\times 0  \\\\ -3 \\times 2 + 0 \\times -3 &-3 \\times 1 + 0 \\times 0 \\end{pmatrix} = \\begin{pmatrix} 1 &2 \\\\ -6 &-3  \\end{pmatrix}  \\neq E\n",
    "\\end{align*}\n",
    "$$\n",
    "\n",
    "so $E$ is not idempotent. \n",
    "\n",
    "$$\n",
    "\\begin{align*}\n",
    "E^T = \\begin{pmatrix} 2 &1 \\\\ -3 &0 \\end{pmatrix}^T = \\begin{pmatrix} 2 &-3 \\\\ 1 &0 \\end{pmatrix} \\neq E^{-1}\n",
    "\\end{align*}\n",
    "$$\n",
    "\n",
    "so $E$ is not orthogonal. \n"
   ]
  },
  {
   "cell_type": "markdown",
   "metadata": {},
   "source": [
    "## Quiz 4\n",
    "\n",
    "### Question 2\n",
    "\n",
    "4 digits, with no digit repeated. The order matters. \n",
    "\n",
    "There are 10 options for the first digit: $\\{ 0, 1, 2, 3, 4, 5, 6, 7, 8, 9 \\}$\n",
    "\n",
    "There are 9 options for the second digit (the numbers above without whatever was chosen first). There are 8 options for the third digit and 7 options for the fourth. \n",
    "\n",
    "Therefore, there are $10 \\times 9 \\times 8 \\times 7$ possible pin codes. \n",
    "\n",
    "\n",
    "### Question 3\n",
    "Each of the 8 teams must play each other team: $8 \\times 7$. But we're counting every game twice, so the answer is $8 \\times 7 / 2$.\n",
    "\n",
    "Alternatively, each game is a combination of two teams from 8 (combination not permutation since the order doesn't matter - team 1 playing team 3 is the same as team 3 playing team 1). This is \n",
    "\n",
    "$$\n",
    "\\begin{align*}\n",
    "8^C_2 = \\frac{8!}{2! 6!} = \\frac{8 \\times 7 \\times 6 \\times 5 \\times 4 \\times 3 \\times 2 \\times 1}{(2 \\times 1) \\times (6 \\times 5 \\times 4 \\times 3 \\times 2 \\times 1)} = \\frac{8 \\times 7}{2}\n",
    "\\end{align*}\n",
    "$$"
   ]
  },
  {
   "cell_type": "code",
   "execution_count": null,
   "metadata": {},
   "outputs": [],
   "source": []
  }
 ],
 "metadata": {
  "kernelspec": {
   "display_name": "R",
   "language": "R",
   "name": "ir"
  },
  "language_info": {
   "codemirror_mode": "r",
   "file_extension": ".r",
   "mimetype": "text/x-r-source",
   "name": "R",
   "pygments_lexer": "r",
   "version": "3.6.1"
  }
 },
 "nbformat": 4,
 "nbformat_minor": 4
}